theories/program_logic.v
@@ -1,14 +1,116 @@
 From machine_program_logic.program_logic Require Import machine weakestpre.
 From HypVeri Require Export lang RAs.
+From iris.proofmode Require Import tactics.
+From iris_string_ident Require Import ltac2_string_ident.
 
-Lemma machine_mixin : MachineMixin terminated HypVeri.lang.step.
+Section lifting.
+
+Lemma machine_mixin : MachineMixin terminated step.
 Proof.
   refine {| mixin_terminated_stuck := terminated_stuck |}.
 Qed.
 
-Canonical Structure hyp_machine := Machine terminated step (Some scheduler) machine_mixin.
+Canonical Structure hyp_machine :=
+  Machine terminated step (Some scheduler) machine_mixin.
 
-Context `{_ : irisG hyp_machine Σ}.
+Context `{_ : !irisG hyp_machine Σ}.
+
+Lemma sswp_lift_step_fupd {i E Φ} m1 :
+  machine.terminated m1 = false →
+  (∀ σ1 , ⌜scheduled σ1 i⌝ -∗  state_interp σ1 ={E,∅}=∗
+    ⌜reducible m1 σ1⌝ ∗
+    ∀ m2 σ2 , ⌜step m1 σ1 m2 σ2 ⌝ ={∅}=∗ ▷ |={∅,E}=>
+      state_interp σ2 ∗  Φ m2 )
+  ⊢ SSWP m1 @ i; E {{ Φ }}.
+Proof.
+  by rewrite sswp_eq /sswp_def=>->.
+Qed.
+
+Lemma sswp_lift_step {i E Φ} m1 :
+  machine.terminated m1 = false →
+  (∀ σ1 , ⌜scheduled σ1 i⌝ -∗  state_interp σ1 ={E,∅}=∗
+    ⌜reducible m1 σ1⌝ ∗
+    ▷∀ m2 σ2 , ⌜step m1 σ1 m2 σ2 ⌝ ={∅,E}=∗
+      state_interp σ2 ∗  Φ m2 )
+  ⊢ SSWP m1 @ i; E {{ Φ }}.
+Proof.
+  iIntros (?) "H".
+  iApply sswp_lift_step_fupd; [done |].
+  iIntros (?) "Hsche Hσ".
+  iMod ("H" $! σ1 with "Hsche Hσ") as "[ $ H]".
+  iIntros "!> * % !> !>".
+  by iApply "H".
+Qed.
 
 
-Lemma mov_reg_rule (i : vmid) : PC @@ i  ⊢ SSWP ExecI @ i {{ (λ m, True) }}%I.
+Lemma sswp_lift_atomic_step_fupd {i E1 E2 Φ} m1 :
+  machine.terminated m1 = false →
+  (∀ σ1 , ⌜scheduled σ1 i⌝ -∗  state_interp σ1 ={E1}=∗
+    ⌜reducible m1 σ1⌝ ∗
+    ∀ m2 σ2 , ⌜step m1 σ1 m2 σ2 ⌝ ={E1} [E2]▷=∗
+      state_interp σ2 ∗  Φ m2 )
+  ⊢ SSWP m1 @ i; E1 {{ Φ }}.
+Proof.
+  iIntros (?) "H".
+  iApply (sswp_lift_step_fupd m1)=>//.
+  iIntros (?) "Hsche Hσ".
+  iMod ("H" $! σ1 with "Hsche Hσ") as "[$ H]".
+  iApply fupd_mask_intro;first set_solver.
+  iIntros "Hclose" (m2 σ2 ?).
+  iMod "Hclose" as "_".
+  iMod ("H" $! m2 σ2 with "[#]") as "H";[done|].
+  iApply fupd_mask_intro;first set_solver.
+  iIntros " Hclose !>".
+  iMod "Hclose" as "_".
+  by iApply "H".
+Qed.
+
+Lemma sswp_lift_atomic_step {i E Φ} m1 :
+  machine.terminated m1 = false →
+  (∀ σ1 , ⌜scheduled σ1 i⌝ -∗  state_interp σ1 ={E}=∗
+    ⌜reducible m1 σ1⌝ ∗
+    ▷ ∀ m2 σ2 , ⌜step m1 σ1 m2 σ2 ⌝ ={E}=∗
+      state_interp σ2 ∗  Φ m2 )
+  ⊢ SSWP m1 @ i; E {{ Φ }}.
+Proof.
+  iIntros (?) "H".
+  iApply (@sswp_lift_atomic_step_fupd i E E Φ);[done|].
+  iIntros (??) "Hσ".
+  iMod ("H" $! σ1 H0 with "Hσ") as "[$ H]".
+  iIntros "!> *".
+  iIntros (Hstep).
+  do 2 iModIntro.
+  by iApply "H".
+Qed.
+
+End lifting.
+
+Section rules.
+
+Global Instance hyp_irisG `{gen_VMG Σ}: irisG hyp_machine Σ:=
+  {
+  iris_invG := gen_invG;
+  state_interp := gen_vm_interp
+  }.
+
+Context `{vmG: !gen_VMG Σ}.
+Implicit Type a : addr.
+Implicit Type i : vmid.
+Implicit Type ra rb : reg_name.
+Implicit Type w: word.
+Implicit Type q : Qp.
+
+
+
+
+Lemma mov_word {i w1 w3 q} a w2 ra :
+  decode_instruction w1 = Some(Mov ra (inl w2)) ->
+  PC @@ i ->r a ∗ a ->a w1 ∗ A@i:={q} (mm_translation a) ∗ ra @@ i ->r w3  ⊢ SSWP ExecI @ i {{ (λ m, True) }}%I.
+Proof.
+  iIntros (Hdecode) "(Hpc & Hapc & Hacc & Hra)".
+  iApply (sswp_lift_atomic_step ExecI);[done|].
+  iIntros (σ1) "%Hsche Hσ".
+  simplify_eq /=.
+  iModIntro.
+  (*TODO:  need some helper lemmas ...*)
+  Admitted.
